formal/isabelle/TRUST12_OBSTRUCTIONS/TRUST_State_Interaction_Controls.thy
@@ -1,0 +1,193 @@
+theory TRUST_State_Interaction_Controls
+ imports TRUST_Structure_Invariant_Controls
+begin
+
+definition sc_initial_100 where
+ "sc_initial_100 = native_initial_state 1 100 1 1 (\<lambda>_. obstruction_binding) 0"
+definition sc_seize_case where
+ "sc_seize_case n amount c = obstruction_seize\<lparr>forward_action_id := n, forward_nonce := n, forward_amount := amount, forward_case := c\<rparr>"
+definition sc_custody_first where
+ "sc_custody_first = forward_success_state sc_initial_100 (sc_seize_case 1 40 1) (obstruction_witness (sc_seize_case 1 40 1))"
+definition sc_custody_two where
+ "sc_custody_two = forward_success_state sc_custody_first (sc_seize_case 2 60 2) (obstruction_witness (sc_seize_case 2 60 2))"
+definition sc_custody_one_released where
+ "sc_custody_one_released = reversal_success_state sc_custody_two (sc_reverse 3 1 TRUST_RELEASE)
+   (sc_reversal_witness sc_custody_two (sc_reverse 3 1 TRUST_RELEASE))"
+lemmas custody_interaction_compute = sc_initial_100_def sc_seize_case_def sc_custody_first_def
+ sc_custody_two_def sc_custody_one_released_def reversal_control_compute
+
+lemma first_shared_custodian_seize_admitted:
+ "forward_admitted sc_initial_100 1 1 (sc_seize_case 1 40 1) (obstruction_witness (sc_seize_case 1 40 1))"
+ by (simp add: custody_interaction_compute forward_admitted_def forward_shape_wf_def forward_fresh_def forward_nonce_key_def
+   forward_authorized_def authority_admits_def forward_current_dependency_def forward_in_window_def within_window_def
+   receipt_matches_forward_def transfer_shape_def no_disposition_commitments_def terminal_case_def open_case_def
+   unbacked_available_def forward_external_commitment_def)
+lemma second_shared_custodian_seize_admitted:
+ "forward_admitted sc_custody_first 1 1 (sc_seize_case 2 60 2) (obstruction_witness (sc_seize_case 2 60 2))"
+ by (simp add: custody_interaction_compute forward_admitted_def forward_shape_wf_def forward_fresh_def forward_nonce_key_def
+   forward_authorized_def authority_admits_def forward_current_dependency_def forward_in_window_def within_window_def
+   receipt_matches_forward_def transfer_shape_def no_disposition_commitments_def terminal_case_def open_case_def
+   unbacked_available_def forward_external_commitment_def)
+lemma one_of_two_custody_releases_admitted:
+ "reversal_admitted sc_custody_two 1 1 (sc_reverse 3 1 TRUST_RELEASE) (sc_reversal_witness sc_custody_two (sc_reverse 3 1 TRUST_RELEASE))"
+ by (simp add: custody_interaction_compute reversal_control_admission)
+
+theorem shared_custodian_release_control_linked:
+ "linked_run sc_initial_100
+   [sc_forward_step sc_initial_100 (sc_seize_case 1 40 1), sc_forward_step sc_custody_first (sc_seize_case 2 60 2),
+    sc_reverse_step sc_custody_two (sc_reverse 3 1 TRUST_RELEASE)] sc_custody_one_released"
+ using forward_control_is_model_step[OF first_shared_custodian_seize_admitted]
+   forward_control_is_model_step[OF second_shared_custodian_seize_admitted]
+   reversal_control_is_model_step[OF one_of_two_custody_releases_admitted]
+ by (simp add: sc_forward_step_def sc_reverse_step_def sc_custody_first_def sc_custody_two_def sc_custody_one_released_def)
+
+theorem shared_custodian_release_preserves_other_case:
+ "physical_balances sc_custody_one_released 1 = 40 \<and> physical_balances sc_custody_one_released 2 = 60 \<and>
+   custody_backing sc_custody_one_released 2 = 60 \<and>
+   map_option custody_active (custody_records sc_custody_one_released 1) = Some False \<and>
+   map_option custody_active (custody_records sc_custody_one_released 2) = Some True \<and>
+   map_option custody_amount (custody_records sc_custody_one_released 2) = Some 60 \<and>
+   map_option custody_action (custody_records sc_custody_one_released 2) = Some (Some 2) \<and>
+   abstract_lifecycle (record_at sc_custody_one_released 2) = Record_Applied"
+ by (simp add: custody_interaction_compute)
+
+theorem shared_custodian_release_control_wf:
+ "\<exists>A C. {1} \<subseteq> A \<and> state_wf A C sc_custody_one_released"
+proof -
+ have INIT: "state_wf {1} {} sc_initial_100" unfolding sc_initial_100_def by (rule native_initial_state_wf)
+ show ?thesis using linked_run_preserves_state_wf[OF INIT shared_custodian_release_control_linked] by blast
+qed
+
+definition corrupt_second_custody where
+ "corrupt_second_custody transform = sc_custody_one_released\<lparr>custody_records := (custody_records sc_custody_one_released)
+   (2 := Some (transform (the (custody_records sc_custody_one_released 2))))\<rparr>"
+text \<open>These are invariant-detection fixtures. They are not reachable attacks.\<close>
+theorem wrong_custody_action_is_detected:
+ "\<not> custody_case_wf (corrupt_second_custody (\<lambda>cu. cu\<lparr>custody_action := Some 1\<rparr>))"
+ by (simp add: corrupt_second_custody_def custody_case_wf_def open_case_def custody_interaction_compute; rule exI[where x=2]; simp)
+theorem wrong_custody_holder_is_detected:
+ "\<not> custody_case_wf (corrupt_second_custody (\<lambda>cu. cu\<lparr>custody_prior_holder := 3\<rparr>))"
+ by (simp add: corrupt_second_custody_def custody_case_wf_def open_case_def custody_interaction_compute; rule exI[where x=2]; simp)
+theorem wrong_custody_amount_is_detected:
+ "\<not> custody_case_wf (corrupt_second_custody (\<lambda>cu. cu\<lparr>custody_amount := 59\<rparr>))"
+ by (simp add: corrupt_second_custody_def custody_case_wf_def open_case_def custody_interaction_compute; rule exI[where x=2]; simp)
+
+definition release_without_inactive_zero where
+ "release_without_inactive_zero = sc_custody_one_released\<lparr>custody_records := (custody_records sc_custody_one_released)
+   (1 := Some ((the (custody_records sc_custody_two 1))\<lparr>custody_active := False\<rparr>))\<rparr>"
+theorem inactive_amount_clear_removal_is_detected:
+ "\<not> custody_case_wf release_without_inactive_zero"
+ by (simp add: release_without_inactive_zero_def custody_case_wf_def open_case_def custody_interaction_compute; rule exI[where x=1]; simp)
+
+theorem ordinary_transfer_to_new_support_control:
+ "ordinary_transfer_allowed obstruction_initial 1 3 1 \<and>
+   state_wf {1,3} {} (ordinary_transfer_state obstruction_initial 1 3 1) \<and>
+   \<not> balance_wf {1} (ordinary_transfer_state obstruction_initial 1 3 1)"
+proof -
+ have AD: "ordinary_transfer_allowed obstruction_initial 1 3 1"
+   by (simp add: ordinary_transfer_allowed_def ordinary_available_def required_floor_def own_frozen_floor_def obstruction_compute)
+ have WF: "state_wf {1,3} {} (ordinary_transfer_state obstruction_initial 1 3 1)"
+   using ordinary_transfer_preserves_state_wf[OF control_initial_state_wf AD] by (simp add: insert_commute)
+ show ?thesis using AD WF by (simp add: balance_wf_def ordinary_transfer_state_def obstruction_compute)
+qed
+
+theorem allowed_self_transfer_control:
+ "ordinary_transfer_allowed obstruction_initial 1 1 1 \<and> ordinary_transfer_state obstruction_initial 1 1 1 = obstruction_initial"
+proof -
+ have AD: "ordinary_transfer_allowed obstruction_initial 1 1 1"
+   by (simp add: ordinary_transfer_allowed_def ordinary_available_def required_floor_def own_frozen_floor_def obstruction_compute)
+ show ?thesis using AD ordinary_self_transfer_stutters[OF AD] by simp
+qed
+
+definition sc100_freeze where
+ "sc100_freeze n amount c = (sc_freeze n amount)\<lparr>forward_case := c\<rparr>"
+definition sc100_first where
+ "sc100_first = forward_success_state sc_initial_100 (sc100_freeze 1 60 1) (obstruction_witness (sc100_freeze 1 60 1))"
+definition sc100_second where
+ "sc100_second = forward_success_state sc100_first (sc100_freeze 2 140 1) (obstruction_witness (sc100_freeze 2 140 1))"
+definition sc100_parent where
+ "sc100_parent = reversal_success_state sc100_second (sc_reverse 3 2 TRUST_UNFREEZE) (sc_reversal_witness sc100_second (sc_reverse 3 2 TRUST_UNFREEZE))"
+definition sc100_clear where
+ "sc100_clear = reversal_success_state sc100_parent (sc_reverse 4 1 TRUST_UNFREEZE) (sc_reversal_witness sc100_parent (sc_reverse 4 1 TRUST_UNFREEZE))"
+definition sc100_restart where
+ "sc100_restart = forward_success_state sc100_clear (sc100_freeze 5 80 5) (obstruction_witness (sc100_freeze 5 80 5))"
+lemmas history_interaction_compute = sc100_freeze_def sc100_first_def sc100_second_def sc100_parent_def
+ sc100_clear_def sc100_restart_def custody_interaction_compute
+lemmas forward_control_admission = forward_admitted_def forward_shape_wf_def forward_fresh_def forward_nonce_key_def
+ reversal_nonce_key_def forward_authorized_def authority_admits_def forward_current_dependency_def forward_in_window_def
+ within_window_def receipt_matches_forward_def overlay_shape_def no_disposition_commitments_def overlay_admissible_def
+ terminal_case_def forward_external_commitment_def
+
+lemma below_supply_freeze_control_admitted:
+ "forward_admitted sc_initial_100 1 1 (sc100_freeze 1 60 1) (obstruction_witness (sc100_freeze 1 60 1))"
+ by (simp add: forward_control_admission history_interaction_compute)
+lemma crossed_supply_freeze_control_admitted:
+ "forward_admitted sc100_first 1 1 (sc100_freeze 2 140 1) (obstruction_witness (sc100_freeze 2 140 1))"
+ by (simp add: forward_control_admission history_interaction_compute)
+lemma crossed_supply_parent_pop_admitted:
+ "reversal_admitted sc100_second 1 1 (sc_reverse 3 2 TRUST_UNFREEZE) (sc_reversal_witness sc100_second (sc_reverse 3 2 TRUST_UNFREEZE))"
+ by (simp add: reversal_control_admission history_interaction_compute)
+lemma crossed_supply_root_pop_admitted:
+ "reversal_admitted sc100_parent 1 1 (sc_reverse 4 1 TRUST_UNFREEZE) (sc_reversal_witness sc100_parent (sc_reverse 4 1 TRUST_UNFREEZE))"
+ by (simp add: reversal_control_admission history_interaction_compute)
+lemma new_case_after_two_pops_admitted:
+ "forward_admitted sc100_clear 1 1 (sc100_freeze 5 80 5) (obstruction_witness (sc100_freeze 5 80 5))"
+ by (simp add: forward_control_admission history_interaction_compute)
+
+theorem crossed_supply_two_pops_new_case_linked:
+ "linked_run sc_initial_100
+   [sc_forward_step sc_initial_100 (sc100_freeze 1 60 1), sc_forward_step sc100_first (sc100_freeze 2 140 1),
+    sc_reverse_step sc100_second (sc_reverse 3 2 TRUST_UNFREEZE), sc_reverse_step sc100_parent (sc_reverse 4 1 TRUST_UNFREEZE),
+    sc_forward_step sc100_clear (sc100_freeze 5 80 5)] sc100_restart"
+ using forward_control_is_model_step[OF below_supply_freeze_control_admitted]
+   forward_control_is_model_step[OF crossed_supply_freeze_control_admitted]
+   reversal_control_is_model_step[OF crossed_supply_parent_pop_admitted]
+   reversal_control_is_model_step[OF crossed_supply_root_pop_admitted]
+   forward_control_is_model_step[OF new_case_after_two_pops_admitted]
+ by (simp add: sc_forward_step_def sc_reverse_step_def sc100_first_def sc100_second_def sc100_parent_def sc100_clear_def sc100_restart_def)
+
+theorem historical_reversed_parent_and_new_head_control:
+ "\<exists>A C. state_wf A C sc100_restart"
+proof -
+ have INIT: "state_wf {1} {} sc_initial_100" unfolding sc_initial_100_def by (rule native_initial_state_wf)
+ show ?thesis using linked_run_preserves_state_wf[OF INIT crossed_supply_two_pops_new_case_linked] by blast
+qed
+
+theorem historical_parent_lifecycle_and_generation_values:
+ "abstract_lifecycle (record_at sc100_restart 1) = Record_Reversed \<and>
+   abstract_lifecycle (record_at sc100_restart 2) = Record_Reversed \<and>
+   effect_parent (link_at sc100_restart 2) = Some 1 \<and>
+   effect_generation (link_at sc100_restart 1) = 1 \<and> head_generation (freeze_heads sc100_restart 1) = 5 \<and>
+   frozen_targets sc100_restart 1 = 80 \<and> case_phase (case_records sc100_restart 1) = Case_Terminal \<and>
+   case_phase (case_records sc100_restart 5) = Case_Open"
+ by (simp add: history_interaction_compute)
+
+definition sc_coexisting_restrict where
+ "sc_coexisting_restrict = (sc_restrict 2)\<lparr>forward_case := 2\<rparr>"
+definition sc_coexisting where
+ "sc_coexisting = forward_success_state sc_one sc_coexisting_restrict (obstruction_witness sc_coexisting_restrict)"
+definition sc_coexisting_unrestricted where
+ "sc_coexisting_unrestricted = reversal_success_state sc_coexisting (sc_reverse 3 2 TRUST_UNRESTRICT)
+   (sc_reversal_witness sc_coexisting (sc_reverse 3 2 TRUST_UNRESTRICT))"
+lemmas coexistence_compute = sc_coexisting_restrict_def sc_coexisting_def sc_coexisting_unrestricted_def reversal_control_compute
+lemma coexisting_restriction_admitted:
+ "forward_admitted sc_one 1 1 sc_coexisting_restrict (obstruction_witness sc_coexisting_restrict)"
+ by (simp add: forward_control_admission restrict_would_not_change_state_def coexistence_compute)
+lemma coexisting_unrestriction_admitted:
+ "reversal_admitted sc_coexisting 1 1 (sc_reverse 3 2 TRUST_UNRESTRICT) (sc_reversal_witness sc_coexisting (sc_reverse 3 2 TRUST_UNRESTRICT))"
+ by (simp add: reversal_control_admission coexistence_compute)
+
+theorem restriction_removal_preserves_coexisting_freeze:
+ "frozen_targets sc_coexisting_unrestricted 1 = 2 \<and> head_action (freeze_heads sc_coexisting_unrestricted 1) = Some 1 \<and>
+   case_phase (case_records sc_coexisting_unrestricted 1) = Case_Open \<and>
+   \<not> restriction_flags sc_coexisting_unrestricted 1 \<and> case_phase (case_records sc_coexisting_unrestricted 2) = Case_Terminal"
+ by (simp add: coexistence_compute)
+
+theorem repeated_restriction_and_other_case_amendment_rejected:
+ "\<not> forward_shape_wf sc_coexisting ((sc_restrict 3)\<lparr>forward_case := 2\<rparr>) \<and>
+   \<not> forward_shape_wf sc_coexisting ((sc_freeze 3 3)\<lparr>forward_case := 3\<rparr>)"
+ by (simp add: forward_shape_wf_def restrict_would_not_change_state_def overlay_shape_def no_disposition_commitments_def
+   overlay_admissible_def terminal_case_def coexistence_compute)
+
+
+end
