formal/isabelle/TRUST12_OBSTRUCTIONS/TRUST_Unfreeze_Preservation.thy
@@ -1,0 +1,396 @@
+theory TRUST_Unfreeze_Preservation
+  imports TRUST_Reversal_Preservation
+begin
+
+lemma unfreeze_context:
+ assumes WF: "regulatory_structure_wf st" and AD: "reversal_admissible st cmd"
+   and KIND: "reversal_kind cmd = TRUST_UNFREEZE"
+ obtains r where "action_records st (reversal_original_action_id cmd) = Some r"
+   and "abstract_action r = Legal_Freeze" and "abstract_lifecycle r = Record_Applied"
+   and "head_action (freeze_heads st (abstract_subject r)) = Some (reversal_original_action_id cmd)"
+   and "frozen_targets st (abstract_subject r) = abstract_amount r"
+   and "open_case st (abstract_case r)"
+   and "case_family (case_records st (abstract_case r)) = Family_Freeze"
+   and "case_head (case_records st (abstract_case r)) = Some (reversal_original_action_id cmd)"
+proof -
+ obtain r where REC: "action_records st (reversal_original_action_id cmd) = Some r"
+   and ACT: "abstract_action r = Legal_Freeze" and APPLIED: "abstract_lifecycle r = Record_Applied"
+   and HD: "head_action (freeze_heads st (abstract_subject r)) = Some (reversal_original_action_id cmd)"
+   and AMOUNT: "frozen_targets st (abstract_subject r) = abstract_amount r"
+   using AD KIND by (auto simp: reversal_admissible_def reversal_original_def reversal_pairs_def
+      reversal_current_effect_def Let_def split: option.splits)
+ have F: "freeze_structure_wf st" using WF unfolding regulatory_structure_wf_def by blast
+ note FA = F[unfolded freeze_structure_wf_def, rule_format, of "abstract_subject r"]
+ have MORE: "open_case st (abstract_case r) \<and> case_family (case_records st (abstract_case r)) = Family_Freeze \<and>
+   case_head (case_records st (abstract_case r)) = Some (reversal_original_action_id cmd)"
+   using FA REC HD by (auto simp: record_at_def)
+ show thesis using that REC ACT APPLIED HD AMOUNT MORE by blast
+qed
+
+lemma unfreeze_state_view:
+ assumes REC: "action_records st (reversal_original_action_id cmd) = Some r"
+   and KIND: "reversal_kind cmd = TRUST_UNFREEZE"
+ shows "reversal_success_state st cmd w = st\<lparr>
+   compositional_consumed_nonces := insert (reversal_nonce_key cmd) (compositional_consumed_nonces st),
+   compositional_receipts := (compositional_receipts st)(reversal_id cmd := Some (reversal_witness_receipt w)),
+   action_records := (action_records st)(reversal_original_action_id cmd := Some (r\<lparr>abstract_lifecycle := Record_Reversed\<rparr>)),
+   frozen_targets := (frozen_targets st)(abstract_subject r := abstract_prior_amount r),
+   freeze_heads := (freeze_heads st)(abstract_subject r := popped_head (freeze_heads st (abstract_subject r)) (link_parent st (reversal_original_action_id cmd))),
+   case_records := (case_records st)(abstract_case r := reopened_or_closed (case_records st (abstract_case r)) (link_parent st (reversal_original_action_id cmd)))\<rparr>"
+ using assms by (simp add: reversal_success_state_def reversal_original_def Let_def)
+
+lemma unfreeze_preserves_action_identity:
+ assumes WF: "regulatory_structure_wf st" and AD: "reversal_admissible st cmd"
+   and KIND: "reversal_kind cmd = TRUST_UNFREEZE"
+ shows "action_identity_wf (reversal_success_state st cmd w)"
+proof -
+ obtain r where REC: "action_records st (reversal_original_action_id cmd) = Some r"
+   and ACT: "abstract_action r = Legal_Freeze" and OPEN: "open_case st (abstract_case r)"
+   using unfreeze_context[OF WF AD KIND] by blast
+ note VIEW = unfreeze_state_view[OF REC KIND, of w]
+ have AI: "action_identity_wf st" using WF unfolding regulatory_structure_wf_def by blast
+ show ?thesis unfolding action_identity_wf_def
+   apply (intro allI impI)
+   subgoal premises P for i q
+   proof (cases "i = reversal_original_action_id cmd")
+     case True
+     note AIR = AI[unfolded action_identity_wf_def, rule_format, of "reversal_original_action_id cmd" r]
+     show ?thesis using P True AIR REC ACT OPEN
+       by (auto simp: VIEW closed_case_def reopened_or_closed_def open_case_def split: option.splits legal_action_kind.splits if_splits)
+   next
+     case False
+     have OLD: "action_records st i = Some q" using P False by (simp add: VIEW)
+     note AIQ = AI[unfolded action_identity_wf_def, rule_format, of i q]
+     show ?thesis using AIQ OLD False REC ACT OPEN
+       by (auto simp: VIEW closed_case_def reopened_or_closed_def open_case_def split: option.splits legal_action_kind.splits if_splits)
+   qed
+   done
+qed
+
+lemma unfreeze_preserves_effect_history:
+ assumes WF: "regulatory_structure_wf st" and AD: "reversal_admissible st cmd"
+   and KIND: "reversal_kind cmd = TRUST_UNFREEZE"
+ shows "effect_history_wf (reversal_success_state st cmd w)"
+proof -
+ obtain r where REC: "action_records st (reversal_original_action_id cmd) = Some r"
+   and ACT: "abstract_action r = Legal_Freeze" and OPEN: "open_case st (abstract_case r)"
+   using unfreeze_context[OF WF AD KIND] by blast
+ note VIEW = unfreeze_state_view[OF REC KIND, of w]
+ have H: "effect_history_wf st" using WF unfolding regulatory_structure_wf_def by blast
+ show ?thesis unfolding effect_history_wf_def
+ proof (intro allI impI)
+   fix i e
+   assume E: "effect_links (reversal_success_state st cmd w) i = Some e"
+   have E0: "effect_links st i = Some e" using E by (simp add: VIEW)
+   note HI = H[unfolded effect_history_wf_def, rule_format, of i e]
+   show "action_records (reversal_success_state st cmd w) i \<noteq> None \<and> i \<noteq> 0 \<and>
+     (let r = record_at (reversal_success_state st cmd w) i in abstract_subject r \<noteq> 0 \<and> abstract_case r \<noteq> 0 \<and>
+       abstract_action r \<in> {Legal_Freeze, Legal_Restrict} \<and> effect_generation e > 0 \<and>
+       effect_generation e \<le> head_generation (if abstract_action r = Legal_Freeze then freeze_heads (reversal_success_state st cmd w) (abstract_subject r)
+         else restriction_heads (reversal_success_state st cmd w) (abstract_subject r)) \<and>
+       (case effect_parent e of None \<Rightarrow> abstract_prior_amount r = 0 \<and> \<not> abstract_prior_flag r
+        | Some j \<Rightarrow> abstract_action r = Legal_Freeze \<and> action_records (reversal_success_state st cmd w) j \<noteq> None \<and>
+          effect_links (reversal_success_state st cmd w) j \<noteq> None \<and> abstract_action (record_at (reversal_success_state st cmd w) j) = Legal_Freeze \<and>
+          abstract_subject (record_at (reversal_success_state st cmd w) j) = abstract_subject r \<and>
+          abstract_case (record_at (reversal_success_state st cmd w) j) = abstract_case r \<and>
+          effect_generation (link_at (reversal_success_state st cmd w) j) < effect_generation e \<and>
+          abstract_prior_amount r = abstract_amount (record_at (reversal_success_state st cmd w) j)))"
+     using HI E0 REC ACT by (auto simp: VIEW record_at_def link_at_def Let_def popped_head_def
+       split: option.splits if_splits; presburger)
+ qed
+qed
+
+lemma unfreeze_pop_context:
+ assumes WF: "regulatory_structure_wf st"
+   and REC: "action_records st i = Some r"
+   and HD: "head_action (freeze_heads st (abstract_subject r)) = Some i"
+ shows "\<exists>xs. distinct (i # xs) \<and> live_freeze_chain st (abstract_subject r) (abstract_case r) (i # xs) \<and>
+   link_parent st i = (case xs of [] \<Rightarrow> None | j # _ \<Rightarrow> Some j) \<and>
+   abstract_prior_amount r = (case xs of [] \<Rightarrow> 0 | j # _ \<Rightarrow> abstract_amount (record_at st j))"
+proof -
+ have AT: "record_at st i = r" using REC by (simp add: record_at_def)
+ show ?thesis using freeze_head_pop_view(1)[OF WF HD] AT by simp
+qed
+
+lemma unfreeze_preserves_freeze_structure:
+ assumes WF: "regulatory_structure_wf st" and AD: "reversal_admissible st cmd"
+   and KIND: "reversal_kind cmd = TRUST_UNFREEZE"
+ shows "freeze_structure_wf (reversal_success_state st cmd w)"
+proof -
+ let ?post = "reversal_success_state st cmd w"
+ let ?id = "reversal_original_action_id cmd"
+ obtain r where REC: "action_records st ?id = Some r"
+   and HD: "head_action (freeze_heads st (abstract_subject r)) = Some ?id"
+   and OPEN: "open_case st (abstract_case r)"
+   and FAMILY: "case_family (case_records st (abstract_case r)) = Family_Freeze"
+   and CASE: "case_head (case_records st (abstract_case r)) = Some ?id"
+   using unfreeze_context[OF WF AD KIND] by blast
+ note VIEW = unfreeze_state_view[OF REC KIND, of w]
+ obtain xs where DIST: "distinct (?id # xs)"
+   and CH: "live_freeze_chain st (abstract_subject r) (abstract_case r) (?id # xs)"
+   and LP: "link_parent st ?id = (case xs of [] \<Rightarrow> None | j # _ \<Rightarrow> Some j)"
+   and PRIOR: "abstract_prior_amount r = (case xs of [] \<Rightarrow> 0 | j # _ \<Rightarrow> abstract_amount (record_at st j))"
+   using unfreeze_pop_context[OF WF REC HD] by blast
+ have TAIL0: "live_freeze_chain st (abstract_subject r) (abstract_case r) xs" using CH by simp
+ have OUT0: "?id \<notin> set xs" using DIST by simp
+ have TAIL: "live_freeze_chain ?post (abstract_subject r) (abstract_case r) xs"
+   by (rule reversal_preserves_chain_away[OF AD TAIL0 OUT0])
+ have F: "freeze_structure_wf st" using WF unfolding regulatory_structure_wf_def by blast
+ show ?thesis unfolding freeze_structure_wf_def
+ proof (intro allI)
+   fix a
+   note FA = F[unfolded freeze_structure_wf_def, rule_format, of a]
+   show "(case head_action (freeze_heads ?post a) of None \<Rightarrow> frozen_targets ?post a = 0
+    | Some i \<Rightarrow> (\<exists>ys. distinct (i # ys) \<and> live_freeze_chain ?post a (abstract_case (record_at ?post i)) (i # ys)) \<and>
+      frozen_targets ?post a = abstract_amount (record_at ?post i) \<and>
+      open_case ?post (abstract_case (record_at ?post i)) \<and>
+      case_family (case_records ?post (abstract_case (record_at ?post i))) = Family_Freeze \<and>
+      case_head (case_records ?post (abstract_case (record_at ?post i))) = Some i)"
+   proof (cases "a = abstract_subject r")
+     case True
+     show ?thesis
+     proof (cases xs)
+       case Nil
+       show ?thesis using True Nil LP PRIOR by (simp add: VIEW popped_head_def)
+     next
+       case (Cons j ys)
+       have NE: "j \<noteq> ?id" using DIST Cons by auto
+       have FIELDS: "abstract_subject (record_at st j) = abstract_subject r \<and> abstract_case (record_at st j) = abstract_case r"
+         using TAIL0 Cons by simp
+       have POST_REC: "record_at ?post j = record_at st j" by (simp add: VIEW record_at_def NE)
+       show ?thesis using True Cons LP PRIOR DIST TAIL FIELDS POST_REC OPEN FAMILY
+         by (auto simp: VIEW popped_head_def reopened_or_closed_def open_case_def record_at_def NE
+           intro!: exI[where x=ys])
+     qed
+   next
+     case False
+     have AA: "a \<noteq> abstract_subject r" by (rule False)
+     show ?thesis
+     proof (cases "head_action (freeze_heads st a)")
+       case None
+       show ?thesis using FA None AA by (simp add: VIEW)
+     next
+       case (Some i)
+       obtain ys where D: "distinct (i # ys)" and OLDCH: "live_freeze_chain st a (abstract_case (record_at st i)) (i # ys)"
+         using FA Some by auto
+       have OUT: "?id \<notin> set (i # ys)"
+       proof
+         assume IN: "?id \<in> set (i # ys)"
+         have "abstract_subject (record_at st ?id) = a" using freeze_chain_member_fields[OF OLDCH IN] by blast
+         then show False using REC AA by (simp add: record_at_def)
+       qed
+       have NE: "i \<noteq> ?id" using OUT by auto
+       have AWAY: "abstract_case (record_at st i) \<noteq> abstract_case r" using FA Some CASE NE by auto
+       have NEWCH: "live_freeze_chain ?post a (abstract_case (record_at st i)) (i # ys)"
+         by (rule reversal_preserves_chain_away[OF AD OLDCH OUT])
+       show ?thesis using FA Some D NEWCH NE AWAY AA
+         by (auto simp: VIEW record_at_def open_case_def cong: option.case_cong intro!: exI[where x=ys])
+     qed
+   qed
+ qed
+qed
+
+lemma unfreeze_preserves_case_structure:
+ assumes WF: "regulatory_structure_wf st" and AD: "reversal_admissible st cmd"
+   and KIND: "reversal_kind cmd = TRUST_UNFREEZE"
+ shows "case_structure_wf (reversal_success_state st cmd w)"
+proof -
+ let ?post = "reversal_success_state st cmd w"
+ let ?id = "reversal_original_action_id cmd"
+ obtain r where REC: "action_records st ?id = Some r"
+   and HD: "head_action (freeze_heads st (abstract_subject r)) = Some ?id"
+   and OPEN: "open_case st (abstract_case r)"
+   and FAMILY: "case_family (case_records st (abstract_case r)) = Family_Freeze"
+   using unfreeze_context[OF WF AD KIND] by blast
+ note VIEW = unfreeze_state_view[OF REC KIND, of w]
+ obtain xs where DIST: "distinct (?id # xs)"
+   and CH: "live_freeze_chain st (abstract_subject r) (abstract_case r) (?id # xs)"
+   and LP: "link_parent st ?id = (case xs of [] \<Rightarrow> None | j # _ \<Rightarrow> Some j)"
+   using unfreeze_pop_context[OF WF REC HD] by blast
+ have C: "case_structure_wf st" using WF unfolding regulatory_structure_wf_def by blast
+ show ?thesis unfolding case_structure_wf_def
+ proof (intro allI)
+   fix c
+   note CC = C[unfolded case_structure_wf_def, rule_format, of c]
+   show "(case case_phase (case_records ?post c) of
+     Case_None \<Rightarrow> case_records ?post c = empty_case
+   | Case_Terminal \<Rightarrow> case_head (case_records ?post c) = None
+   | Case_Open \<Rightarrow> (case case_head (case_records ?post c) of None \<Rightarrow> False | Some i \<Rightarrow>
+      action_records ?post i \<noteq> None \<and> abstract_case (record_at ?post i) = c \<and>
+      (case case_family (case_records ?post c) of
+        Family_Freeze \<Rightarrow> head_action (freeze_heads ?post (abstract_subject (record_at ?post i))) = Some i
+      | Family_Restrict \<Rightarrow> head_action (restriction_heads ?post (abstract_subject (record_at ?post i))) = Some i
+      | Family_Custody \<Rightarrow> abstract_action (record_at ?post i) = Legal_Seize
+      | _ \<Rightarrow> False)))"
+   proof (cases "c = abstract_case r")
+     case True
+     show ?thesis
+     proof (cases xs)
+       case Nil
+       show ?thesis using True Nil LP by (simp add: VIEW reopened_or_closed_def closed_case_def)
+     next
+       case (Cons j ys)
+       have NE: "j \<noteq> ?id" using DIST Cons by auto
+       have FIELDS: "action_records st j \<noteq> None \<and> abstract_subject (record_at st j) = abstract_subject r \<and>
+         abstract_case (record_at st j) = abstract_case r" using CH Cons by simp
+       show ?thesis using True Cons LP NE FIELDS OPEN FAMILY
+         by (auto simp: VIEW reopened_or_closed_def popped_head_def open_case_def record_at_def)
+     qed
+   next
+     case False
+     show ?thesis using CC REC HD False
+       by (auto simp: VIEW reopened_or_closed_def closed_case_def popped_head_def record_at_def empty_case_def
+         cong: option.case_cong trust_case_phase.case_cong trust_case_family.case_cong
+         split: option.splits trust_case_phase.splits trust_case_family.splits if_splits)
+   qed
+ qed
+qed
+
+
+lemma unfreeze_preserves_restriction_structure:
+ assumes WF: "regulatory_structure_wf st" and AD: "reversal_admissible st cmd"
+   and KIND: "reversal_kind cmd = TRUST_UNFREEZE"
+ shows "restriction_structure_wf (reversal_success_state st cmd w)"
+proof -
+ let ?post = "reversal_success_state st cmd w"
+ let ?id = "reversal_original_action_id cmd"
+ obtain r where REC: "action_records st ?id = Some r" and ACT: "abstract_action r = Legal_Freeze"
+   and FAMILY: "case_family (case_records st (abstract_case r)) = Family_Freeze"
+   using unfreeze_context[OF WF AD KIND] by blast
+ note VIEW = unfreeze_state_view[OF REC KIND, of w]
+ have R: "restriction_structure_wf st" using WF unfolding regulatory_structure_wf_def by blast
+ show ?thesis unfolding restriction_structure_wf_def
+ proof (intro allI)
+   fix a
+   note RA = R[unfolded restriction_structure_wf_def, rule_format, of a]
+   show "(case head_action (restriction_heads ?post a) of None \<Rightarrow> \<not> restriction_flags ?post a
+    | Some i \<Rightarrow> restriction_flags ?post a \<and> action_records ?post i \<noteq> None \<and> effect_links ?post i \<noteq> None \<and>
+      abstract_action (record_at ?post i) = Legal_Restrict \<and> abstract_lifecycle (record_at ?post i) = Record_Applied \<and>
+      abstract_subject (record_at ?post i) = a \<and> \<not> abstract_prior_flag (record_at ?post i) \<and>
+      effect_parent (link_at ?post i) = None \<and> open_case ?post (abstract_case (record_at ?post i)) \<and>
+      case_family (case_records ?post (abstract_case (record_at ?post i))) = Family_Restrict \<and>
+      case_head (case_records ?post (abstract_case (record_at ?post i))) = Some i)"
+     using RA REC ACT FAMILY
+     by (auto simp: VIEW popped_head_def closed_case_def reopened_or_closed_def record_at_def link_at_def open_case_def
+       cong: option.case_cong split: option.splits if_splits)
+ qed
+qed
+
+lemma unfreeze_preserves_custody_case:
+ assumes WF: "regulatory_structure_wf st" and AD: "reversal_admissible st cmd"
+   and KIND: "reversal_kind cmd = TRUST_UNFREEZE"
+ shows "custody_case_wf (reversal_success_state st cmd w)"
+proof -
+ let ?post = "reversal_success_state st cmd w"
+ let ?id = "reversal_original_action_id cmd"
+ obtain r where REC: "action_records st ?id = Some r" and ACT: "abstract_action r = Legal_Freeze"
+   and FAMILY: "case_family (case_records st (abstract_case r)) = Family_Freeze"
+   using unfreeze_context[OF WF AD KIND] by blast
+ note VIEW = unfreeze_state_view[OF REC KIND, of w]
+ have CU: "custody_case_wf st" using WF unfolding regulatory_structure_wf_def by blast
+ have CUSTODY_FRAME: "custody_records ?post = custody_records st" by (simp add: VIEW)
+ have CASE_FRAME: "\<And>c. c \<noteq> abstract_case r \<Longrightarrow> case_records ?post c = case_records st c"
+   by (simp add: VIEW)
+ have NO_ACTIVE: "\<not> (\<exists>cu. custody_records st (abstract_case r) = Some cu \<and> custody_active cu)"
+   using CU[unfolded custody_case_wf_def, THEN conjunct1, rule_format, of "abstract_case r"] FAMILY by simp
+ have ACTIVE_AWAY: "\<And>c cu. custody_records st c = Some cu \<Longrightarrow> custody_active cu \<Longrightarrow> c \<noteq> abstract_case r"
+   using NO_ACTIVE by blast
+ have RECORD_FRAME: "\<And>i q. action_records st i = Some q \<Longrightarrow> abstract_action q = Legal_Seize \<Longrightarrow>
+   action_records ?post i = Some q"
+   using REC ACT by (auto simp: VIEW split: option.splits if_splits)
+ have CASE_CUSTODY: "\<And>c. (open_case ?post c \<and> case_family (case_records ?post c) = Family_Custody) =
+   (open_case st c \<and> case_family (case_records st c) = Family_Custody)"
+   using FAMILY by (auto simp: VIEW closed_case_def reopened_or_closed_def open_case_def split: option.splits if_splits)
+ have EQUIV: "\<forall>c. (open_case ?post c \<and> case_family (case_records ?post c) = Family_Custody) =
+   (\<exists>cu. custody_records ?post c = Some cu \<and> custody_active cu)"
+   using CU unfolding custody_case_wf_def by (simp only: CASE_CUSTODY CUSTODY_FRAME; blast)
+ have LINKS: "\<forall>c cu. custody_records ?post c = Some cu \<longrightarrow>
+   (if custody_active cu then
+      (\<exists>i r. custody_action cu = Some i \<and> case_head (case_records ?post c) = Some i \<and>
+       action_records ?post i = Some r \<and> abstract_lifecycle r = Record_Applied \<and> abstract_action r = Legal_Seize \<and>
+       abstract_case r = c \<and> abstract_source r = custody_prior_holder cu \<and> abstract_subject r = custody_prior_holder cu \<and>
+       abstract_destination r = custody_custodian cu \<and> abstract_custodian r = custody_custodian cu \<and>
+       abstract_amount r = custody_amount cu \<and> custody_amount cu > 0 \<and> custody_prior_holder cu \<noteq> 0 \<and>
+       custody_custodian cu \<noteq> 0 \<and> custody_prior_holder cu \<noteq> custody_custodian cu)
+    else custody_amount cu = 0)"
+ proof (intro allI impI)
+   fix c cu
+   assume POST: "custody_records ?post c = Some cu"
+   have OLD: "custody_records st c = Some cu" using POST CUSTODY_FRAME by simp
+   let ?link = "\<lambda>s. \<exists>i r. custody_action cu = Some i \<and> case_head (case_records s c) = Some i \<and>
+       action_records s i = Some r \<and> abstract_lifecycle r = Record_Applied \<and> abstract_action r = Legal_Seize \<and>
+       abstract_case r = c \<and> abstract_source r = custody_prior_holder cu \<and> abstract_subject r = custody_prior_holder cu \<and>
+       abstract_destination r = custody_custodian cu \<and> abstract_custodian r = custody_custodian cu \<and>
+       abstract_amount r = custody_amount cu \<and> custody_amount cu > 0 \<and> custody_prior_holder cu \<noteq> 0 \<and>
+       custody_custodian cu \<noteq> 0 \<and> custody_prior_holder cu \<noteq> custody_custodian cu"
+   have BEFORE: "if custody_active cu then ?link st else custody_amount cu = 0"
+     using CU OLD unfolding custody_case_wf_def by blast
+   show "if custody_active cu then ?link ?post else custody_amount cu = 0"
+   proof (cases "custody_active cu")
+     case False
+     then show ?thesis using BEFORE by simp
+   next
+     case True
+     have AWAY: "c \<noteq> abstract_case r" by (rule ACTIVE_AWAY[OF OLD True])
+     have CS: "case_records ?post c = case_records st c" by (rule CASE_FRAME[OF AWAY])
+     obtain i r where W: "custody_action cu = Some i \<and> case_head (case_records st c) = Some i \<and>
+       action_records st i = Some r \<and> abstract_lifecycle r = Record_Applied \<and> abstract_action r = Legal_Seize \<and>
+       abstract_case r = c \<and> abstract_source r = custody_prior_holder cu \<and> abstract_subject r = custody_prior_holder cu \<and>
+       abstract_destination r = custody_custodian cu \<and> abstract_custodian r = custody_custodian cu \<and>
+       abstract_amount r = custody_amount cu \<and> custody_amount cu > 0 \<and> custody_prior_holder cu \<noteq> 0 \<and>
+       custody_custodian cu \<noteq> 0 \<and> custody_prior_holder cu \<noteq> custody_custodian cu"
+       using BEFORE True by auto
+     have REC: "action_records ?post i = Some r" using RECORD_FRAME W by blast
+     show ?thesis using True W CS REC by auto
+   qed
+ qed
+ show ?thesis using EQUIV LINKS unfolding custody_case_wf_def by blast
+qed
+
+theorem unfreeze_preserves_regulatory_structure:
+ assumes WF: "regulatory_structure_wf st" and AD: "reversal_admissible st cmd"
+   and KIND: "reversal_kind cmd = TRUST_UNFREEZE"
+ shows "regulatory_structure_wf (reversal_success_state st cmd w)"
+ using unfreeze_preserves_action_identity[OF WF AD KIND]
+   unfreeze_preserves_effect_history[OF WF AD KIND]
+   unfreeze_preserves_freeze_structure[OF WF AD KIND]
+   unfreeze_preserves_restriction_structure[OF WF AD KIND]
+   unfreeze_preserves_case_structure[OF WF AD KIND]
+   unfreeze_preserves_custody_case[OF WF AD KIND]
+ unfolding regulatory_structure_wf_def by blast
+
+lemma unfreeze_preserves_accounting_state_wf:
+ assumes WF: "state_wf A C st" and AD: "reversal_admissible st cmd"
+   and KIND: "reversal_kind cmd = TRUST_UNFREEZE"
+ shows "accounting_state_wf A C (reversal_success_state st cmd w)"
+proof -
+ let ?post = "reversal_success_state st cmd w"
+ have AC: "accounting_state_wf A C st" and REG: "regulatory_structure_wf st"
+   using WF unfolding state_wf_def by blast+
+ obtain r where REC: "action_records st (reversal_original_action_id cmd) = Some r"
+   and OPEN: "open_case st (abstract_case r)"
+   using unfreeze_context[OF REG AD KIND] by blast
+ note VIEW = unfreeze_state_view[OF REC KIND, of w]
+ have IN: "abstract_case r \<in> C"
+   using AC OPEN by (auto simp: accounting_state_wf_def case_scope_def open_case_def empty_case_def)
+ have BAL: "balance_wf A ?post" using AC by (simp add: accounting_state_wf_def balance_wf_def VIEW)
+ have SCOPE: "case_scope C ?post" using AC IN by (auto simp: accounting_state_wf_def case_scope_def VIEW)
+ have CU_FRAME: "custody_consistent C ?post = custody_consistent C st"
+   by (simp add: custody_consistent_def active_custody_sum_def VIEW)
+ have CU: "custody_consistent C ?post" using AC CU_FRAME unfolding accounting_state_wf_def by blast
+ have REF: "custody_case_wf ?post" by (rule unfreeze_preserves_custody_case[OF REG AD KIND])
+ show ?thesis using BAL SCOPE CU REF unfolding accounting_state_wf_def by blast
+qed
+
+theorem unfreeze_preserves_state_wf:
+ assumes WF: "state_wf A C st" and AD: "reversal_admitted st sender time cmd w"
+   and KIND: "reversal_kind cmd = TRUST_UNFREEZE"
+ shows "state_wf A C (reversal_success_state st cmd w)"
+proof -
+ have ADM: "reversal_admissible st cmd" using AD by (simp add: reversal_admitted_def)
+ have REG: "regulatory_structure_wf st" using WF by (simp add: state_wf_def)
+ show ?thesis using unfreeze_preserves_accounting_state_wf[OF WF ADM KIND]
+   unfreeze_preserves_regulatory_structure[OF REG ADM KIND] unfolding state_wf_def by blast
+qed
+
+end
